edit common

Common.v
@@ -13,28 +13,7 @@ Import ListNotations.
 
 Section MachineModel.
   Definition var : Type := nat.
-  
-  Definition condition : Type := nat.
-  Inductive location : Type :=
-  | Not_cnd : nat -> location
-  | Cnd : condition -> location.
-  Definition is_Cnd (l: location) : Prop :=
-    match l with
-    | Not_cnd _ => False
-    | Cnd _ => True
-    end.
-  Definition is_Not_cnd (l: location) : Prop :=
-    match l with
-    | Not_cnd _ => True
-    | Cnd _ => False
-    end.
-  Definition locations_eq l1 l2: bool :=
-    match l1, l2 with
-    | Not_cnd n, Not_cnd n' => n =? n'
-    | Cnd c, Cnd c' => c =? c'
-    | _, _ => false
-    end.
-
+  Definition location : Type := nat.
   Definition register (value_t: Type) : Type := var -> value_t.
   Definition memory (value_t: Type) : Type := location -> value_t.
 End MachineModel.
@@ -42,158 +21,48 @@ End MachineModel.
 Section Security.
   Inductive sec_level : Set :=
   | L : sec_level
-  | H : sec_level
-  | T : sec_level.
-
-  Inductive sec_level_rel : relation sec_level :=
-  | sec_level_l_rel : sec_level_rel L H
-  | sec_level_h_rel : sec_level_rel H T.
-
-  (*
-  Definition sec_level_le := clos_refl_trans sec_level sec_level_rel.
-  
-  Global Instance sec_level_le_refl : Reflexive sec_level_le.
-  intro sl; destruct sl; unfold sec_level_le; apply rt_refl.
-  Defined.
-
-  Global Instance sec_level_le_trans : Transitive sec_level_le.
-  intros sl1 sl2 sl3;  unfold sec_level_le; intros.
-  apply rt_trans with (y:=sl2); auto.
-  Defined.
-
-  Lemma sec_level_le_dec : forall sl sl', {sec_level_le sl sl'} + {sec_level_le sl' sl}.
-  Proof.
-    intros; destruct sl, sl'; intuition;
-      [left|left|right|left|right|right]; unfold sec_level_le.
-    apply rt_step; apply sec_level_l_rel.
-    apply rt_trans with (y := H); apply rt_step; [apply sec_level_l_rel | apply sec_level_h_rel].
-    apply rt_step; apply sec_level_l_rel.
-    apply rt_step; apply sec_level_h_rel.
-    apply rt_trans with (y := H); apply rt_step; [apply sec_level_l_rel | apply sec_level_h_rel].
-    apply rt_step; apply sec_level_h_rel.
-  Qed.
-   *)
+  | H : sec_level.
 
   Definition sec_level_le (sl sl': sec_level) :=
     match sl, sl' with
-    | H, L | T, L | T, H => False
+    | H, L  => False
     | _, _ => True
     end.
 
   Definition sec_level_le_compute (sl sl': sec_level) :=
     match sl, sl' with
-      | H, L | T, L | T, H => false
+      | H, L  => false
       | _, _ => true
     end.
   Lemma sec_level_le_correct (sl sl': sec_level) :
     sec_level_le_compute sl sl' = true <-> sec_level_le sl sl'.
   Proof.
     destruct sl, sl'; intuition; try discriminate; unfold sec_level_le in *; auto.
-  Admitted.
+  Qed.
 
   Definition sec_level_join (sl sl': sec_level) : sec_level :=
     match sl, sl' with
-    | T, _ | _, T => T
     | H, _ | _, H => H
     | L, L => L
     end.
-
   Lemma sec_level_join_ge (sl sl': sec_level) :
     sec_level_le sl (sec_level_join sl sl') /\ sec_level_le sl' (sec_level_join sl sl').
   Proof.
     induction sl, sl'; unfold sec_level_join; unfold sec_level_le; auto.
   Qed.
-
   Lemma sec_level_le_trans (sl sl' sl'': sec_level) :
     sec_level_le sl sl' -> sec_level_le sl' sl'' -> sec_level_le sl sl''.
   Proof.
     intros; unfold sec_level_le; induction sl, sl', sl''; auto.
   Qed.
-
   Lemma sec_level_le_refl (sl : sec_level) :
     sec_level_le sl sl.
   Proof.
     intros; unfold sec_level_le; induction sl; auto.
   Qed.
-  
-  Inductive sec_policy : Type :=
-  | LevelP : sec_level -> sec_policy
-  | ErasureP (l1: sec_level) (cnd: condition) (l2: sec_level)
-             (l1_le_l2: sec_level_le l1 l2) : sec_policy.
-  
-  Definition sec_spec : Type :=  location -> sec_policy.
 
-  Definition well_formed_spec (g : sec_spec) : Prop :=
-    forall l, exists p, g l = p /\ p <> LevelP T /\ forall cnd sl pf, p <> ErasureP T cnd sl pf.
+  Definition sec_spec : Type :=  location -> sec_level.
+  Definition well_formed_spec (g : sec_spec) : Prop := forall l, exists p, g l = p.
 
-  Inductive policy_le : relation sec_policy :=
-  | PLE1 : forall l1 l2,
-      sec_level_le l1 l2 ->
-      policy_le (LevelP l1) (LevelP l2)
-  | PLE2 : forall p1 l2 l2' cnd pf,
-      policy_le p1 (LevelP l2) ->
-      policy_le p1 (ErasureP l2 cnd l2' pf)
-  | PLE3 : forall l1 l1' p2 cnd pf,
-      policy_le (LevelP l1') p2 ->
-      policy_le (ErasureP l1 cnd l1' pf) p2
-  | PLE4 : forall l1 l1' l2 l2' cnd pf1 pf2,
-      sec_level_le l1 l2 ->
-      sec_level_le l1' l2' ->
-      policy_le (ErasureP l1 cnd l1' pf1) (ErasureP l2 cnd l2' pf2).
-
-  Lemma policy_le_refl : reflexive sec_policy policy_le.
-  Proof.
-    intro x. destruct x.
-    - apply PLE1. apply sec_level_le_refl.
-    - apply PLE4; apply sec_level_le_refl.
-  Qed.
-
-  Lemma policy_le_antisymmetric : antisymmetric sec_policy policy_le.
-  Proof.
-  Admitted.
-
-  Lemma policy_le_transitive : transitive sec_policy policy_le.
-  Proof.
-  Admitted.
-  
-  Lemma policy_le_partial_order : order sec_policy policy_le.
-  Proof.
-    split.
-    - apply policy_le_refl.
-    - apply policy_le_transitive.
-    - apply policy_le_antisymmetric.
-  Qed.  
- 
-  Parameter policy_join : sec_policy -> sec_policy -> sec_policy.
-  Axiom policy_le_join : forall p1 p2,
-      policy_le p1 (policy_join p1 p2) /\ policy_le p2 (policy_join p1 p2).
-  Axiom policy_le_join_inv : forall p1 p2 p,
-      policy_le (policy_join p1 p2) p -> policy_le p1 p /\ policy_le p2 p.
-  
-  Function cur (p : sec_policy) (U : set condition) : sec_level :=
-    match p with
-    | LevelP l => l
-    | ErasureP l1 cnd l2 _ => if (set_mem Nat.eq_dec cnd U) then l1 else l2
-    end.
-
-  Inductive protected : sec_policy -> Prop :=
-  | level_high: protected (LevelP H)
-  | level_top: protected (LevelP T)
-  (*
-  | erase_high: forall cnd sl pf,
-      protected (ErasureP H cnd sl pf)*)
-  | join_protected_l: forall p p',
-      protected p ->
-      protected (policy_join p p')
-  | join_protected_r: forall p p',
-      protected p' ->
-      protected (policy_join p p').
-
-  Lemma protected_gt_L : forall p, protected p -> sec_level_le (cur p []) L = False.
-  Proof.
-    intros.
-    induction H0; simpl; auto.
-    admit.
-    admit.
-  Admitted.
+  Definition protected (sl: sec_level) : Prop := sl = H.      
 End Security.
